

ECE210 - Homework 13

Due: Wednesday, December 5, 2018 at 6:00 p.m.

1. For each one of the 4 signals $f(t)$ in parts (a), (b), (c), (d), do the following

- i. Obtain its Laplace transform $\hat{F}(s)$.
- ii. Indicate the poles of $\hat{F}(s)$.
- iii. Indicate the ROC of $\hat{F}(s)$.

- (a) $f(t) = u(t-6) - u(t+6)$
- (b) $f(t) = te^{2(t-1)}u(t)$
- (c) $f(t) = (t-1)e^{-4t} + \delta(t)$
- (d) $f(t) = e^{2t} \cos(t-1)u(t+1)$.

Solution:

- (a) $f(t) = u(t-6) - u(t+6)$

i. Using the Laplace transform definition, we have

$$\hat{F}(s) = \int_{0^-}^{\infty} [u(t-6) - u(t+6)] e^{-st} dt = \int_{0^-}^6 -e^{-st} dt = \frac{-1 + e^{-6s}}{s}.$$

ii. poles:

Testing if $\hat{F}(s) \rightarrow \pm\infty$ as $s \rightarrow 0$: $\lim_{s \rightarrow 0} \hat{F}(s) = \lim_{s \rightarrow 0} \frac{-1 + e^{-6s}}{s} = \frac{0}{0}$ (indeterminate). Applying l'Hospital rule we find out that $s = 0$ is not a pole, because $\lim_{s \rightarrow 0} \hat{F}(s) \neq \pm\infty$:

$$\lim_{s \rightarrow 0} \frac{-1 + e^{-6s}}{s} = \lim_{s \rightarrow 0} \frac{\frac{d}{ds}(-1 + e^{-6s})}{\frac{d}{ds}(s)} = \lim_{s \rightarrow 0} \frac{-6e^{-6s}}{1} = -6 \neq \infty.$$

There is a set of poles as $\text{Re}\{s\} \rightarrow -\infty$. Therefore, we say that there is a "hidden" pole at $s = -\infty + j\omega$.
List of poles:

$$s_1 = \{-\infty + j\omega\}.$$

iii. We recognize the ROC as the region to the right of the rightmost pole: $\sigma = \text{Re}\{s\} > -\infty$.

- (b) $f(t) = te^{2(t-1)}u(t) = e^{-2}te^{2t}u(t)$

i. Using Laplace transform tables we obtain

$$\hat{F}(s) = \frac{e^{-2}}{(s-2)^2},$$

ii. list of poles: $s_{1,2} = 2$ (double pole)iii. ROC: $\sigma = \text{Re}\{s\} > 2$.This means that this Laplace integral converges only for values of s such that $\text{Re}\{s\} > 2$.

- (c) $f(t) = (t-1)e^{-4t} + \delta(t) = te^{-4t} - e^{-4t} + \delta(t)$

i. Using Laplace transform tables we obtain

$$\hat{F}(s) = \frac{1}{(s+4)^2} - \frac{1}{s+4} + 1 = \frac{s^2 + 7s + 13}{(s+4)^2} = \frac{\left(s - \frac{-7+j\sqrt{55}}{2}\right)\left(s - \frac{-7-j\sqrt{55}}{2}\right)}{(s+4)^2}.$$

ii. list of poles: $s_{1,2} = \{-4\}$ (double)iii. ROC: $\sigma = \text{Re}\{s\} > -4$.This means that this Laplace integral converges only for values of s such that $\text{Re}\{s\} > -4$.

(d) $f(t) = e^{3t} \cos(t-1)u(t-1)$

- i. The Laplace transform starts at $t = 0$. Therefore it will be the same as calculating the L.T of $f(t) = e^{2t} \cos(t-1)u(t)$. Using Table 11.1, we obtain

$$f(t) = e^3 e^{3(t-1)} \cos(t-1)u(t-1) \longleftrightarrow \hat{F}(s) = e^{(3-s)} \frac{s-3}{(s-(3+j))(s-(3-j))}.$$

- ii. There is a set of poles as $\text{Re}\{s\} \rightarrow -\infty$. Therefore, list of poles: $s_{1,2} = \{3+j, 3-j\}$ and $s_3 = \{-\infty + j\omega\}$.
 iii. ROC: $\sigma = \text{Re}\{s\} > 3$.

This means that this Laplace integral converges only for values of s such that $\text{Re}\{s\} > 3$.

2. Determine whether the LTIC systems with the following transfer functions are BIBO stable and explain why or why not.

(a) $\hat{H}_1(s) = 2 + \frac{s}{(s-1)(s+2)}$

(b) $\hat{H}_2(s) = \frac{s^2+5s+6}{(s-1+j5)(s-1-j5)}$

(c) $\hat{H}_3(s) = \frac{s^3+1}{(s+2)(s+4)}$

(d) $\hat{H}_4(s) = \frac{1}{s^2+16}$

(e) $\hat{H}_5(s) = \frac{s-2}{s^2-4}$.

Solution:

- (a) $\hat{H}_1(s)$ has a pole in the RHP at $s = 1$, so the system is not BIBO stable.
 (b) $\hat{H}_2(s)$ has two conjugate poles at $s = 1-j5$, and $s = 1 + j5$, both in the RHP, so the system is not BIBO stable.
 (c) $\hat{H}_3(s)$ has two poles at $s = -2$, $s = -4$ and $s = +\infty$. Because the pole at infinity is not confined to the LHP, the system is not BIBO stable.
 (d) $\hat{H}_4(s)$ has two conjugate poles on the imaginary axis at $s = j4$, and $s = -j4$. The system is marginally stable, but not BIBO stable.
 (e) $\hat{H}_5(s)$ has one pole at $s = -2$, so the system is BIBO stable. The unstable pole is cancelled with the unstable zeros.

3. For each of the following Laplace transforms $\hat{F}(s)$, determine the inverse Laplace transform $f(t)$.

(a) $\hat{F}(s) = \frac{s+3}{(s+2)(s+4)}$

(b) $\hat{F}(s) = \frac{1}{s(s-5)^2}$

(c) $\hat{F}(s) = \frac{s^2+2s+1}{(s+1)(s+2)}$

Solution:

- (a) Expressing as a PFE,

$$\hat{F}(s) = \frac{K_1}{(s+2)} + \frac{K_2}{(s+4)}$$

Applying the cover-up method, we have

$$K_1 = 0.5, K_2 = 0.5, \text{ therefore,}$$

$$f(t) = \left(\frac{1}{2}e^{-4t} + \frac{1}{2}e^{-2t}\right) u(t).$$

- (b) Expressing as a PFE,

$$\hat{F}(s) = \frac{1}{s(s-5)^2} = \frac{K_1}{s} + \frac{K_2}{(s-5)^2} + \frac{K_3}{(s-5)}$$

Applying the cover-up method, we have

$$K_1 = \frac{1}{25}, K_2 = \frac{1}{5}, \text{ and } K_3 = -\frac{1}{25}, \text{ therefore,}$$

$$f(t) = \left(\frac{1}{25} + \frac{1}{5}te^{5t} - \frac{1}{25}e^{5t}\right) u(t).$$

- (c) We first simplify the expression by writing

$$\hat{F}(s) = \frac{s^2+2s+1}{(s+1)(s+2)} = \frac{(s+1)(s+2)-(s+1)}{(s+1)(s+2)} = 1 - \frac{1}{(s+2)}$$

Consequently, $f(t) = \delta(t) - e^{-2t}u(t)$.